Cslib/Languages/LambdaCalculus/LocallyNameless/Niit/Basic.lean
@@ -1,0 +1,87 @@
+/-
+Copyright (c) 2025 Chris Henson. All rights reserved.
+Released under Apache 2.0 license as described in the file LICENSE.
+Authors: Thomas Waring
+-/
+
+import Cslib.Languages.LambdaCalculus.LocallyNameless.Context
+import Cslib.Languages.LambdaCalculus.LocallyNameless.Untyped.Properties
+import Mathlib.Data.List.Sigma
+
+/-! # Non-idempotent intersection types
+
+A presentation of non-idempotent intersection types (Niit) for the lambda calculus, using the
+locally nameless presentation.
+
+### References
+
+- See slides <https://pageperso.lis-lab.fr/~giulio.guerrieri/ECI2024/day4.pdf>
+-/
+
+universe u v
+
+variable {Var : Type u} {Base : Type v} [DecidableEq Var]
+
+open LambdaCalculus.LocallyNameless.Untyped Term
+
+namespace LambdaCalculus.LocallyNameless.Niit
+
+inductive LTy (Base : Type v)
+  /-- Base type -/
+  | base : Base → LTy Base
+  /-- Arrow type -/
+  | arrow : List (LTy Base) → LTy Base → LTy Base
+
+inductive Ty (Base : Type v)
+  /-- Linear types -/
+  | lin : LTy Base → Ty Base
+  /-- Multitypes -/
+  | multi : List (LTy Base) → Ty Base
+
+scoped infixr:70 " ⊸ " => LTy.arrow
+
+open LTy Ty Context List
+
+inductive Typing : Term Var → Ty Base → Context Var (List (LTy Base)) → Type _
+  /-- Variables are typed with a sigleton -/
+  | var {x : Var} {A : LTy Base} : Typing (fvar x) (lin A) [⟨x,[A]⟩]
+  /-- Abstractions are typed with arrows, multitypes in argument position, linear in output -/
+  | abs {M : List (LTy Base)} {Γ : Context Var (List (LTy Base))} {A : LTy Base}
+      (t : Term Var) (L : Finset Var) :
+    (∀ x ∉ L, Typing (t ^ fvar x) (lin A) (⟨x,M⟩ :: Γ)) → Typing t.abs  (lin <| M ⊸ A) Γ
+  /-- Application -/
+  | app {Γ Δ : Context Var (List (LTy Base))} {M : List (LTy Base)} {A : LTy Base}
+      {s t : Term Var} :
+    Typing s (lin <| M ⊸ A) Γ → Typing t (multi M) Γ → Typing (app s t) (lin A) (Γ ++ Δ)
+  /-- Bang rule -/
+  | bang {t : Term Var} :
+      (Tys : List (LTy Base × Context Var (List <| LTy Base))) →
+      (Ders : ∀ τ ∈ Tys, Typing t (lin τ.1) τ.2) →
+    Typing t (multi <| Tys.map Prod.fst) (Tys.map Prod.snd).flatten
+  -- Q: does this need permutation rule(s)
+
+scoped notation:50 Γ " ⊢' " t " ∶ " A:arg => Typing t A Γ
+
+variable {Γ : Context Var (List (LTy Base))} {A C : LTy Base}
+
+[HasFresh Var]
+
+example (D : Typing (abs (bvar 0)) (lin C) Γ) : ∃ B : LTy Base, C = [B] ⊸ B := by
+  cases D
+  case abs M A L h =>
+    replace h := h (fresh L) (fresh_notMem L)
+    simp only [open', openRec, ↓reduceIte] at h
+    cases h
+    use A
+
+-- example (D : Typing (abs (app (bvar 0) (bvar 0))) (lin C) Γ) :
+--     ∃ (M : List (LTy Base)) (B : LTy Base), C = ((M ⊸ B) :: M) ⊸ B := by
+--   cases D
+--   case abs N A L h =>
+--     replace h := h (fresh L) (fresh_notMem L)
+--     cases h
+
+
+end Niit
+
+end LambdaCalculus.LocallyNameless
