Cslib/Languages/LambdaCalculus/LocallyNameless/Untyped/HeadBeta.lean
@@ -1,0 +1,111 @@
+/-
+Copyright (c) 2025 Chris Henson. All rights reserved.
+Released under Apache 2.0 license as described in the file LICENSE.
+Authors: Thomas Waring, Chris Henson
+-/
+
+import Cslib.Languages.LambdaCalculus.LocallyNameless.Untyped.FullBeta
+
+/-!
+# Head β reduction
+-/
+
+universe u
+
+variable {Var : Type u}
+
+namespace LambdaCalculus.LocallyNameless.Untyped.Term
+
+/-- A single β-reduction step. -/
+@[reduction_sys headBetaRs "βʰ"]
+inductive HeadBeta : Term Var → Term Var → Prop
+/-- Reduce an application to a lambda term. -/
+| beta : LC (abs M) → LC N → HeadBeta (app (abs M) N) (M ^ N)
+/-- Reduce a redex under an abstraction. -/
+| abs (xs : Finset Var) : (∀ x ∉ xs, HeadBeta (M ^ fvar x) (N ^ fvar x)) →
+    HeadBeta (abs M) (abs N)
+| app : LC Z → ¬ M.Value → HeadBeta M N → HeadBeta (app M Z) (app N Z)
+
+namespace HeadBeta
+
+attribute [scoped grind] app
+
+variable {M M' N N' : Term Var}
+
+@[scoped grind _=_]
+private lemma headBetaRs_Red_eq : M ⭢βʰ N ↔ HeadBeta M N := by
+  have : (@headBetaRs Var).Red = HeadBeta := by rfl
+  simp_all
+
+/-- The left side of a reduction is locally closed. -/
+@[scoped grind →]
+lemma step_lc_l (step : M ⭢βʰ M') : LC M := by
+  induction step <;> constructor
+  all_goals assumption
+
+variable [HasFresh Var] [DecidableEq Var]
+
+omit [HasFresh Var] in
+
+/-- Head reduction is a subrelation of full beta reduction. -/
+lemma full_of_headBeta (step : M ⭢βʰ N) : M ⭢βᶠ N := by
+  induction step
+  case abs m n xs h ih =>
+    apply FullBeta.abs (free_union Var)
+    simpa
+  all_goals constructor <;> first | grind | assumption
+
+/-- Head reduction is deterministic. -/
+lemma headBeta_deterministic (step : M ⭢βʰ N) (step' : M ⭢βʰ N') : N = N' := by
+  induction step generalizing N'
+  <;> cases step'
+  case abs.abs m n xs step ih n' xs' hn' =>
+    congr
+    have ⟨fresh, _⟩ := fresh_exists <| free_union [fv] Var
+    suffices n ^ fvar fresh = n' ^ fvar fresh by
+      apply open_injective (x := fresh) <;> grind
+    grind
+  all_goals grind
+
+/-- The right side of a reduction is locally closed. -/
+@[scoped grind →]
+lemma step_lc_r (step : M ⭢βʰ M') : LC M' := by
+  induction step
+  case' abs => constructor; assumption
+  all_goals grind
+
+/-- Substitution respects a single reduction step. -/
+lemma redex_subst_cong (s s' : Term Var) (x y : Var) (step : s ⭢βʰ s') :
+    s [ x := fvar y ] ⭢βʰ s' [ x := fvar y ] := by
+  induction step
+  case beta m n abs_lc n_lc =>
+    cases abs_lc with | abs xs _ mem =>
+      rw [subst_open x (fvar y) n m (by grind)]
+      refine beta ?_ (by grind)
+      exact subst_lc (LC.abs xs m mem) (LC.fvar y)
+  case abs m' m xs mem ih =>
+    apply abs (free_union Var)
+    grind
+  case app z m n z_lc hm_val h ih =>
+    cases m <;> grind
+
+/-- Abstracting then closing preserves a single reduction. -/
+lemma step_abs_close {x : Var} (step : M ⭢βʰ M') : M⟦0 ↜ x⟧.abs ⭢βʰ M'⟦0 ↜ x⟧.abs := by
+  apply abs ∅
+  grind [redex_subst_cong]
+
+/-- Abstracting then closing preserves multiple reductions. -/
+lemma redex_abs_close {x : Var} (step : M ↠βʰ M') : (M⟦0 ↜ x⟧.abs ↠βʰ M'⟦0 ↜ x⟧.abs) :=  by
+  induction step using Relation.ReflTransGen.trans_induction_on
+  case refl => rfl
+  case single ih => exact Relation.ReflTransGen.single (step_abs_close ih)
+  case trans l r => exact .trans l r
+
+/-- Multiple reduction of opening implies multiple reduction of abstraction. -/
+theorem redex_abs_cong (xs : Finset Var) (cofin : ∀ x ∉ xs, (M ^ fvar x) ↠βʰ (M' ^ fvar x)) :
+    M.abs ↠βʰ M'.abs := by
+  have ⟨fresh, _⟩ := fresh_exists <| free_union [fv] Var
+  rw [open_close fresh M 0 ?_, open_close fresh M' 0 ?_]
+  all_goals grind [redex_abs_close]
+
+end LambdaCalculus.LocallyNameless.Untyped.Term.HeadBeta
